breaking apart the definition of domains & cleanup
code cleanup in abstract interpretation.

src/Analyze/AbstractInterpCpsK.v
@@ -1,10 +1,7 @@
 Require Import String List Bool.
-Require Import CoqCompile.CpsK.
-Require Import ExtLib.Structures.Maps.
+Require Import CoqCompile.CpsK CoqCompile.Analyze.AbstractDomains.
 Require Import ExtLib.Structures.Monads.
 Require Import ExtLib.Structures.Reducible.
-Require Import ExtLib.Data.Monads.ReaderMonad.
-Require Import ExtLib.Data.Monads.StateMonad.
 Require Import ExtLib.Data.Option.
 Require Import ExtLib.Data.Lists.
 Require Import ExtLib.Core.RelDec.
@@ -13,65 +10,14 @@ Require Import ExtLib.Data.Map.FMapAList.
 
 Import CpsK.CPSK.
 
-Section AbstractDomain.
-  
-  Class AbsTime (C : Type) : Type :=
-  { ED :> RelDec (@eq C)
-    (** What does this have? 
-     ** - there should be a way to refine a context to include some pure fact, e.g.
-     **   "assume this equality"
-     ** - there should also be a way to record a stack of call sites for context
-     **   analysis
-     **)
-  }.
-  
-  Class AbsDomain (Domain Value Context ProgramPoint : Type) : Type :=
-  { lookup  : Context -> ProgramPoint -> Domain -> Value
-  ; update  : Context -> ProgramPoint -> Value -> Domain -> Domain
-  ; joinA   : Value -> Value -> Value
-  ; bottomA : Value (** this means empty, i.e. never has a value **)
-  ; topA    : Value (** this means anything of any type **)
-  ; dom_leq   : Domain -> Domain -> bool
-  }.
-
-  Class IntValue (V : Type) : Type :=
-  { injInt : option BinNums.Z -> V
-  ; plusA  : V -> V -> V
-  ; minusA : V -> V -> V
-  ; timesA : V -> V -> V
-  ; eqA    : V -> V -> option bool
-  ; ltA    : V -> V -> option bool
-  }.
-
-  Class BoolValue (V : Type) : Type :=
-  { injBool : option bool -> V
-  ; may : V -> bool -> bool
-  ; must : V -> bool -> bool
-  ; orA : V -> V -> V
-  }.
-
-  Class FnValue (V C D : Type) (exp : Type) : Type :=
-  { injFn  : C -> list cont -> list var -> exp -> V 
-  ; applyA : forall {m} {_ : Monad m}, (C -> D -> exp -> m D%type) -> D -> V -> list V -> list V -> m D%type
-  }.
-
-  Class TplValue (V : Type) : Type :=
-  { injTuple : list V -> V
-  ; projA    : V -> V -> V
-  }.
-
-End AbstractDomain.
-
-(** NOTE: This is poorly coded
- ** Don't use a random second monad to be cool
- **)
 Section AI.
   Variables D C V : Type.
   Context {AbsTime_C  : AbsTime C}.
   Context {AbsValue_V : AbsDomain D V C (var + cont)}.
   Context {IntValue_V : IntValue V}.
   Context {BoolValue_V : BoolValue V}.
-  Context {FnValue_V  : FnValue V C D exp}.
+  Context {CtorValue_V  : CtorValue V constructor}.
+  Context {FnValue_V  : FnValue V C D}.
   Context {TplValue_V : TplValue V}.
 
   Import MonadNotation.
@@ -86,182 +32,104 @@ Section AI.
     (** DFS **)
     Context {State_m : MonadState (alist (C * exp) D) m}.
 
-    Definition m' : Type -> Type := 
-      readerT C (stateT D m).
-
-    Definition runM' {A} (cmd : m' A) (c : C) (d : D) : m (A * D) :=
-      runStateT (runReaderT cmd c) d.
-    
-    Definition eval_op (o : op) : m' V :=
+    Definition eval_op (o : op) (ctx : C) (dom : D) : m V :=
       match o with
         | Var_o v =>
-          domain <- get ;;
-          ctx <- ask ;;
-          ret (lookup ctx (inl v) domain)
+          ret (lookup ctx (inl v) dom)
         | Con_o c => ret bottomA (** TODO: Not done **)
         | Int_o i => ret (injInt (Some i))
         | InitWorld_o => ret bottomA (** TODO: ?? **)
       end.
     
-    Section Transfer.
-      Definition illFormed_decl {A} (d : decl) : m A :=
-        raise ("Ill-formed declaration " ++ runShow (show d))%string.
-      
-      Definition eval_decl (d : decl) : m' unit :=
-        v_vA <- 
-        match d return m' (var * V) with
-          | Op_d v o =>
-            oA <- eval_op o ;;
-            ret (v, oA)
+    Definition illFormed_decl {A} (d : decl) : m A :=
+      raise ("Ill-formed declaration " ++ runShow (show d))%string.
+
+    Definition eval_decl (d : decl) (ctx : C) (dom : D) : m D :=
+      v_vA <- 
+      match d return m (list (var * V)) with
+        | Op_d v o =>
+          oA <- eval_op o ctx dom ;;
+          ret ((v, oA) :: nil)
             
-          | Prim_d v p os => 
-            argsA <- mapM eval_op os ;;
-            vA <- match p , argsA return m' V with
-                    | Eq_p , l :: r :: nil =>
-                      ret (injBool (eqA l r))
-                    | Neq_p , l :: r :: nil =>
-                      ret (injBool (map negb (eqA l r)))
-                    | Lt_p , l :: r :: nil =>
-                      ret (injBool (ltA l r))
-                    | Lte_p , l :: r :: nil =>
-                      ret (orA (injBool (ltA l r)) (injBool (eqA l r)))
-                    | Ptr_p , l :: nil => ret (injBool None) (** ?? **)
-                    | Plus_p , l :: r :: nil => ret (plusA l r)
-                    | Minus_p , l :: r :: nil => ret (minusA l r)
-                    | Times_p , l :: r :: nil => ret (timesA l r)
-                    | MkTuple_p , argsA => ret (injTuple argsA)
-                    | Proj_p , l :: r :: nil => ret (projA l r)
-                    | _ , _ => lift (lift (illFormed_decl (Prim_d v p os)))
-                  end ;;
-            ret (v, vA)
+        | Prim_d v p os => 
+          argsA <- mapM (fun x => eval_op x ctx dom) os ;;
+          vA <- match p , argsA with
+                  | Eq_p , l :: r :: nil =>
+                    ret (injBool (eqA l r))
+                  | Neq_p , l :: r :: nil =>
+                    ret (injBool (map negb (eqA l r)))
+                  | Lt_p , l :: r :: nil =>
+                    ret (injBool (ltA l r))
+                  | Lte_p , l :: r :: nil =>
+                    ret (orA (injBool (ltA l r)) (injBool (eqA l r)))
+                  | Ptr_p , l :: nil => ret (injBool None) (** ?? **)
+                  | Plus_p , l :: r :: nil => ret (plusA l r)
+                  | Minus_p , l :: r :: nil => ret (minusA l r)
+                  | Times_p , l :: r :: nil => ret (timesA l r)
+                  | MkTuple_p , argsA => ret (injTuple argsA)
+                  | Proj_p , l :: r :: nil => ret (projA l r)
+                  | _ , _ => illFormed_decl (Prim_d v p os)
+                end ;;
+          ret ((v, vA) :: nil)
 
-          | Fn_d v ks args body =>
-            ctx <- ask ;;
-            ret (v, injFn ctx ks args body)
-            
-          | Bind_d v1 v2 m os =>
-            ret (v1, topA)
-            (*              
-            argsA <- mapM eval_op os ;;
-            admit
-            r <- bindA aeval m argsA ;;
-            match r with
-              | (a1,a2) =>
-                insert v1 a1 ;;
-                insert v2 a2
-            end
-            *)
-        end ;;
-        let '(v, vA) := v_vA in
-        ctx <- ask (T := C) ;;
-        modify (update ctx (inl v) vA) ;;
-        ret tt.
+        | Fn_d v ks args body =>
+          ret ((v, injFn ctx ks args body) :: nil)
+          
+        | Bind_d v1 v2 m os =>
+          ret ((v1, topA) :: (v2, topA) :: nil)
+      end ;;
+      let dom' := fold_left (fun dom v_vA => let '(v, vA) := v_vA in
+        update ctx (inl v) vA dom) v_vA dom in
+      ret dom'.
 
-      Definition init_decl (d : decl) : m' unit :=
-        ctx <- ask (T := C) ;;
-        match d return m' _ with
-          | Op_d v _ 
-          | Prim_d v _ _
-          | Fn_d v _ _ _ => 
-            modify (update ctx (inl v) bottomA)
-          | Bind_d v1 v2 _ _ =>
-            modify (update ctx (inl v1) bottomA) ;;
-            modify (update ctx (inl v2) bottomA)
-        end ;;
-        ret tt.
+    Definition init_decl (d : decl) (ctx : C) (dom : D) : D :=
+      match d with
+        | Op_d v _ 
+        | Prim_d v _ _
+        | Fn_d v _ _ _ => 
+          update ctx (inl v) bottomA dom
+        | Bind_d v1 v2 _ _ =>
+          let dom := update ctx (inl v1) bottomA dom in
+            update ctx (inl v2) bottomA dom
+      end.
       
-      Definition aeval : C -> D -> exp -> m D :=
-        mfix3 _ (fun aeval => 
-          fun (ctx : C) (dom : D) (e : exp) =>
-            memo <- gets (Maps.lookup (ctx, e)) ;;
-            let stop :=
-              match memo with
-                | None => false
-                | Some dom' => dom_leq dom dom'
-              end
-            in
-            if stop then ret dom
-              else
-                (fix recur (ctx : C) (dom : D) (e : exp) : m D :=
-                  match e return m D with
-                    | App_e o ks os =>
-                      let argsK := List.map (fun k => lookup ctx (inr k) dom) ks in
-                        fA_argsA_d <- runM' (fA <- eval_op o ;;
-                          argsA <- mapM eval_op os ;;
-                          ret (fA, argsK, argsA)) ctx dom ;;
-                        let '((fA, argsK, argsA), dom) := fA_argsA_d in
-                          applyA aeval dom fA argsK argsA 
-                    | Let_e d e =>
-                      v_dom <- runM' (eval_decl d) ctx dom ;;
-                      let '(v, dom) := v_dom in
-                        recur ctx dom e
-                    | AppK_e k os =>
-                      fA_argsA_d <- runM' (let fA := lookup ctx (inr k) dom in
-                        argsA <- mapM eval_op os ;;
-                        ret (fA, argsA)) ctx dom ;;
-                      let _ : ((V * list V) * D) := fA_argsA_d in
-                        let '((fA, argsA), dom)  := fA_argsA_d in
-                          applyA aeval dom fA nil argsA 
-                    | LetK_e ks e =>
-                      dom' <- runM' 
-                      (iterM (fun kxse => let '(k,xs,e) := kxse in
-                        modify (update ctx (inr k) (injFn ctx nil xs e)) ;;
-                        ret tt) ks) ctx dom ;;
-                      recur ctx (snd dom') e
-                    | Letrec_e ds e =>
-                      dom' <- runM' 
-                      (iterM init_decl ds ;;
-                        iterM eval_decl ds) ctx dom ;;
-                      recur ctx (snd dom') e
-                    | Switch_e o arms e =>
-                      s <- runM' (eval_op o) ctx dom ;;
-                      dom' <- foldM (fun x dom => 
-                        ctx <- ret ctx ;;
-                        recur ctx dom (snd x)) (ret dom) arms ;;
-                      match e with
-                        | Some e =>
-                          recur ctx dom' e
-                        | None => ret dom'
-                      end
-                    | Halt_e o1 o2 =>
-                      ret dom
-                  end) ctx dom e).
-
-(*
-        Definition aeval : C -> D -> exp -> m D :=
-          mfix3 _ (fun aeval => fix recur (ctx : C) (dom : D) (e : exp) : m D :=
+    Definition aeval_exp : C -> D -> exp -> m D :=
+      mfix3 _ (fun aeval => fun (ctx : C) (dom : D) (e : exp) =>
+        memo <- gets (Maps.lookup (ctx, e)) ;;
+        let stop :=
+          match memo with
+            | None => false
+            | Some dom' => dom_leq dom dom'
+          end
+        in
+        if stop then ret dom
+        else
+          (fix recur (ctx : C) (dom : D) (e : exp) : m D :=
             match e return m D with
               | App_e o ks os =>
                 let argsK := List.map (fun k => lookup ctx (inr k) dom) ks in
-                fA_argsA_d <- runM' (fA <- eval_op o ;;
-                                     argsA <- mapM eval_op os ;;
-                                     ret (fA, argsK, argsA)) ctx dom ;;
-                let '((fA, argsK, argsA), dom) := fA_argsA_d in
+                fA <- eval_op o ctx dom ;;
+                argsA <- mapM (fun x => eval_op x ctx dom) os ;;
                 applyA aeval dom fA argsK argsA 
               | Let_e d e =>
-                v_dom <- runM' (eval_decl d) ctx dom ;;
-                let '(v, dom) := v_dom in
-                recur ctx dom e
+                dom' <- eval_decl d ctx dom ;;
+                recur ctx dom' e
               | AppK_e k os =>
-                fA_argsA_d <- runM' (let fA := lookup ctx (inr k) dom in
-                                     argsA <- mapM eval_op os ;;
-                                     ret (fA, argsA)) ctx dom ;;
-                let _ : ((V * list V) * D) := fA_argsA_d in
-                let '((fA, argsA), dom)  := fA_argsA_d in
+                let fA := lookup ctx (inr k) dom in
+                argsA <- mapM (fun x => eval_op x ctx dom) os ;;
                 applyA aeval dom fA nil argsA 
               | LetK_e ks e =>
-                dom' <- runM' 
-                  (iterM (fun kxse => let '(k,xs,e) := kxse in
-                    modify (update ctx (inr k) (injFn ctx nil xs e)) ;;
-                    ret tt) ks) ctx dom ;;
-                recur ctx (snd dom') e
+                let dom' := 
+                  fold_left (fun dom kxse => let '(k,xs,e) := kxse in
+                    update ctx (inr k) (injFn ctx nil xs e) dom) ks dom in
+                recur ctx dom' e
               | Letrec_e ds e =>
-                dom' <- runM' 
-                  (iterM init_decl ds ;;
-                   iterM eval_decl ds) ctx dom ;;
-                recur ctx (snd dom') e
+                let dom_init := 
+                  fold_left (fun dom d => init_decl d ctx dom) ds dom in
+                dom' <- foldM (fun d dom => eval_decl d ctx dom) (ret dom_init) ds ;;
+                recur ctx dom' e
               | Switch_e o arms e =>
-                s <- runM' (eval_op o) ctx dom ;;
+                s <- eval_op o ctx dom ;;
                 dom' <- foldM (fun x dom => 
                   ctx <- ret ctx ;;
                   recur ctx dom (snd x)) (ret dom) arms ;;
@@ -272,10 +140,24 @@ Section AI.
                 end
               | Halt_e o1 o2 =>
                 ret dom
-            end).
-*)
-    End Transfer.
+            end) ctx dom e).
     
-  End Monadic.    
+  End Monadic.
+
+  Require Import ExtLib.Data.Monads.EitherMonad.
+  Require Import ExtLib.Data.Monads.StateMonad.
+  Require Import ExtLib.Data.Monads.FuelMonad.
+
+  Section interface.
+    Variable m : Type -> Type.
+    Context {Monad_m : Monad m}.
+    Context {MonadFix_m : MonadFix m}.
+
+    Arguments aeval_exp {m} {_ _ _ _} ctx dom e.
+
+    Definition aeval (ctx : C) (dom : D) (e : exp) : m (string + D) :=
+      let c := aeval_exp (m := eitherT string (stateT (alist (C * exp) D) m)) ctx dom e in 
+      evalStateT (unEitherT c) Maps.empty.
+  End interface.
 
 End AI.
