src/Analyze/AbstractDomains.v
@@ -1,0 +1,60 @@
+Require Import CoqCompile.CpsK.
+Require Import ExtLib.Structures.Monads.
+Require Import ExtLib.Core.RelDec.
+
+Import CpsK.CPSK.
+
+Section AbstractDomain.
+  
+  Class AbsTime (C : Type) : Type :=
+  { ED :> RelDec (@eq C)
+    (** What does this have? 
+     ** - there should be a way to refine a context to include some pure fact, e.g.
+     **   "assume this equality"
+     ** - there should also be a way to record a stack of call sites for context
+     **   analysis
+     **)
+  }.
+  
+  Class AbsDomain (Domain Value Context ProgramPoint : Type) : Type :=
+  { lookup  : Context -> ProgramPoint -> Domain -> Value
+  ; update  : Context -> ProgramPoint -> Value -> Domain -> Domain
+  ; joinA   : Value -> Value -> Value
+  ; bottomA : Value (** this means empty, i.e. never has a value **)
+  ; topA    : Value (** this means anything of any type **)
+  ; dom_leq   : Domain -> Domain -> bool
+  }.
+
+  Class IntValue (V : Type) : Type :=
+  { injInt : option BinNums.Z -> V
+  ; plusA  : V -> V -> V
+  ; minusA : V -> V -> V
+  ; timesA : V -> V -> V
+  ; eqA    : V -> V -> option bool
+  ; ltA    : V -> V -> option bool
+  }.
+
+  Class CtorValue (V : Type) (Ctor : Type) : Type :=
+  { injCtor : Ctor -> V
+  ; isPtrA  : V -> option bool
+  ; ceqA    : V -> V -> option bool
+  }.
+
+  Class BoolValue (V : Type) : Type :=
+  { injBool : option bool -> V
+  ; may : V -> bool -> bool
+  ; must : V -> bool -> bool
+  ; orA : V -> V -> V
+  }.
+
+  Class FnValue (V C D : Type) : Type :=
+  { injFn  : C -> list cont -> list var -> exp -> V 
+  ; applyA : forall {m} {_ : Monad m}, (C -> D -> exp -> m D%type) -> D -> V -> list V -> list V -> m D%type
+  }.
+
+  Class TplValue (V : Type) : Type :=
+  { injTuple : list V -> V
+  ; projA    : V -> V -> V
+  }.
+
+End AbstractDomain.
